# Definition
Seien $M_1, ..., M_\ell$ $R$-[[Modul|Moduln]] mit $(M_i, 0_i, +_i, \cdot_i)$, dann ist der $R$-Modul $$\bigoplus_{i=1}^\ell M_i = \left(\bigtimes_{i=1}^\ell M_i, (0_i)_{i \in \{1, ..., \ell\}} +, \cdot \right)$$ gegeben durch der komponentenweise [[Addition]]
$$+ :\bigoplus_{i=1}^\ell M_i \times \bigoplus_{i=1}^\ell M_i \to \bigoplus_{i=1}^\ell M_i,$$
$$(m, m') \mapsto (m_i)_{i \in \{1, ..., \ell\}} + (m'_i)_{i \in \{1, ..., \ell\}} = (m_i +_i m'_i)_{i \in \{1, ..., \ell\}}$$
bzw. [[Multiplikation]]
$$\cdot :\bigoplus_{i=1}^\ell M_i \times \bigoplus_{i=1}^\ell M_i \to \bigoplus_{i=1}^\ell M_i,$$
$$(m, m') \mapsto (m_i)_{i \in \{1, ..., \ell\}} \cdot (m'_i)_{i \in \{1, ..., \ell\}} = (m_i \cdot_i m'_i)_{i \in \{1, ..., \ell\}}$$

# Beispiel Schreibweise
$$R^n := \bigoplus_{1 \leq i \leq n} R_i$$
$$V_n(R) = \bigoplus_{i=1}^nR = R^n$$