$$\binom nk = \frac{n!}{k!(n-k)!}$$
## [[Binomischer Lehrsatz]]
$${\begin{aligned}(x+y)^{n}&={\binom {n}{0}}x^{n}+{\binom {n}{1}}x^{n-1}y+\dotsb +{\binom {n}{n-1}}xy^{n-1}+{\binom {n}{n}}y^{n}\\&=\sum _{k=0}^{n}{\binom {n}{k}}x^{n-k}y^{k}\end{aligned}}$$
# Eigenschaften
$${\binom {n}{0}}=1={\binom {n}{n}}$$
$${\binom {n}{1}}=n={\binom {n}{n-1}}$$
$${\displaystyle {\binom {n}{k}}={\frac {n-k+1}{k}}{\binom {n}{k-1}}}$$
$${\binom {n}{k}}={\frac {n}{k}}\cdot {\binom {n-1}{k-1}}\Leftrightarrow k\cdot {\binom {n}{k}}=n\cdot {\binom {n-1}{k-1}}$$
$${\binom {n+1}{k+1}}={\binom {n}{k}}+{\binom {n}{k+1}}$$
